I've changed the way tail-recursive functions are defined. They are now defined based on a step function:
  step: 'a -> 'a + 'b

Tail-recursive functions loop until their step function 
returns something in the right component (INR).

examples/machine-code/compiler/compilerLib.sig
@@ -3,11 +3,24 @@ sig
 
   include Abbrev
 
-  (* input : target ("arm", "ppc" or "x86") and term (equation defining function) *)
+  (* supported targets are "arm", "ppc" and "x86" *)
 
+  (* mc_define defines a function and puts the definition on a queue
+     waiting to be compiled, returns function definition and pre *)
+  val mc_define        : term quotation -> thm * thm
+
+  (* mc_compile fname target: compiles function fname to target code,
+     returns a Hoare triple containing the generated code *)
+  val mc_compile       : string -> string -> thm
+
+  (* mc_compile_all fname: compiles function fname to all targets *)
+  val mc_compile_all   : string -> (string * thm) list
+
+  (* these functions expose the back-end functions *)
   val compile      : string -> term -> thm * thm * thm
   val compile_all  : term -> (string * thm) list * thm * thm
 
+  (* the tactic used for proving function equivalence *)
   val COMPILER_TAC : tactic
 
 end
