examples/machine-code/hoare-triple/progScript.sml
@@ -238,5 +238,13 @@ val SPEC_TAILREC = store_thm("SPEC_TAILREC",
   NTAC 9 STRIP_TAC THEN HO_MATCH_MP_TAC TAILREC_PRE_INDUCT
   THEN METIS_TAC [TAILREC_THM,UNION_IDEMPOT,SPEC_COMPOSE]);
 
+val SPEC_SHORT_TAILREC = store_thm("SPEC_SHORT_TAILREC",
+  ``!(f:'a -> ('a + 'b) # bool) res res' c m.
+      (!x y. ISL (FST (f x)) /\ SND (f x) /\ (y = OUTL (FST (f x))) ==> SPEC m (res x) c (res y)) /\
+      (!x y. ~ISL (FST (f x)) /\ SND (f x) /\ (y = OUTR (FST (f x))) ==> SPEC m (res x) c (res' y)) ==>
+      (!x. SHORT_TAILREC_PRE f x ==> SPEC m (res x) c (res' (SHORT_TAILREC f x)))``,
+  SIMP_TAC std_ss [SHORT_TAILREC_PRE_def,SHORT_TAILREC_def] \\ NTAC 6 STRIP_TAC
+  \\ MATCH_MP_TAC SPEC_TAILREC \\ ASM_SIMP_TAC std_ss []);
+
 
 val _ = export_theory();
